Sealing (experiment): Adjust spec context + n types, rather than one type. Ugly.

theories/heap_lang/lib/sealing.v
@@ -31,118 +31,71 @@ Local Notation ext R := (pointwise_relation _ R).
 Module Import intf.
 
 (** Operations *)
-Class SealingImpl : Set := {
-  make_sealer_unsealer : val; seal : val; unseal : val
-}.
-Arguments make_sealer_unsealer _ : clear implicits.
-Arguments seal _ : clear implicits.
-Arguments unseal _ : clear implicits.
+Class SealingImpl : Set := { make_seal : val }.
 
 Section spec.
   Context `{heapG Σ} {SI : SealingImpl}.
   Implicit Types v f : val.
 
-  Definition to_low (φ : val → iProp Σ) : iProp Σ :=
-    (□ ∀ v, φ v -∗ low v)%I.
-  Definition from_low (φ : val → iProp Σ) : iProp Σ :=
-    (□ ∀ v, low v -∗ φ v)%I.
-
   Structure sealing := Sealing {
     (** Predicates. *)
-    (** Name ties [is_sealer_unsealer] to [is_sealed]. *)
+    (** Name ties together the abstract predicates. *)
     name : Type;
-    is_sealer_unsealer (N : namespace) (γ : name) (v : val)
-      (φ : val → iProp Σ) : iProp Σ;
-    is_sealed (N : namespace) (γ : name) (v v' : val) : iProp Σ;
+    is_sealing (γ : name) (φ : val → iProp Σ) : iProp Σ;
+    is_seal (γ : name) (v : val) : iProp Σ;
+    is_unseal (γ : name) (v : val) : iProp Σ;
+    is_sealed (γ : name) (v v' : val) : iProp Σ;
     (** Structure *)
-    is_sealer_unsealer_persistent N γ v φ :
-      PersistentP (is_sealer_unsealer N γ v φ);
-    is_sealer_unsealer_ne N γ v n :
-      Proper (ext (dist n) ==> dist n) (is_sealer_unsealer N γ v);
-    is_sealed_persistent N γ v v' : PersistentP (is_sealed N γ v v');
+    is_sealing_persistent γ φ : PersistentP (is_sealing γ φ);
+    is_sealing_ne γ n : Proper (ext (dist n) ==> dist n) (is_sealing γ);
+    is_seal_persistent γ v : PersistentP (is_seal γ v);
+    is_unseal_persistent γ v : PersistentP (is_unseal γ v);
+    is_sealed_persistent γ v v' : PersistentP (is_sealed γ v v');
+    (** Properties of sealing *)
+    is_seal_low γ s φ :
+      is_sealing γ φ -∗ □ (∀ v, low v -∗ φ v) -∗ is_seal γ s -∗ low s;
+    (** Properties of unsealing *)
+    is_unseal_low γ u φ :
+      is_sealing γ φ -∗ □ (∀ v, φ v -∗ low v) -∗ is_unseal γ u -∗ low u;
     (** Operations *)
-    make_sealer_unsealer_spec N p φ `{Hφ : ∀ v, PersistentP (φ v)} :
+    make_seal_spec N p φ :
       heapN ⊥ N →
-      {{{ heap_ctx }}} make_sealer_unsealer SI () @ p; ⊤
-      {{{ v γ, RET v; is_sealer_unsealer N γ v φ }}};
-    seal_spec N p γ s φ `{Hφ : ∀ v, PersistentP (φ v)} :
-      {{{ is_sealer_unsealer N γ s φ }}} seal SI s @ p; ⊤ {{{ f, RET f;
-        □ (from_low φ -∗ low f) ∗ ∀ p v,
-        {{{ φ v }}} f v @ p; ⊤ {{{ v', RET v'; low v' ∗ is_sealed N γ v v' }}}
+      {{{ heap_ctx }}} make_seal () @ p; ⊤
+      {{{ v1 v2 γ, RET (v1, v2); is_sealing γ φ ∗ is_seal γ v1 ∗ is_unseal γ v2
       }}};
-    unseal_sealed_spec N p γ s φ :
-      {{{ is_sealer_unsealer N γ s φ }}} unseal SI s @ p; ⊤ {{{ f, RET f;
-        ∀ p v v', {{{ is_sealed N γ v v' }}} f v' @ p; ⊤ {{{ RET v; φ v }}}
-      }}};
-    unseal_low_spec N p γ s φ :
-      {{{ is_sealer_unsealer N γ s φ }}} unseal SI s @ p; ⊤ {{{ f, RET f;
-        □ (to_low φ -∗ low f) ∗ ∀ v', {{{ low v' }}} f v' ?{{{ v, RET v; φ v }}}
-      }}}
+    seal_spec p γ s v φ `{!PersistentP (φ v)} :
+      {{{ is_sealing γ φ ∗ is_seal γ s ∗ φ v }}} s v @ p; ⊤
+      {{{ v', RET v'; low v' ∗ is_sealed γ v v' }}};
+    unseal_spec p γ u v v' φ :
+      {{{ is_sealing γ φ ∗ is_unseal γ u ∗ is_sealed γ v v' }}}
+        u v' @ p; ⊤
+      {{{ RET v; φ v }}};
+    unseal_low_spec γ u v' φ :
+      {{{ is_sealing γ φ ∗ is_unseal γ u ∗ low v' }}} u v'
+      ?{{{ v, RET v; φ v }}}
   }.
 End spec.
 Arguments sealing _ {_ _}.
-Existing Instances is_sealer_unsealer_persistent is_sealer_unsealer_ne
-  is_sealed_persistent.
+Existing Instances is_sealing_persistent is_sealing_ne
+  is_seal_persistent is_unseal_persistent is_sealed_persistent.
 
-Section lemmas.
+Section theory.
   Context `{heapG Σ, SI : SealingImpl} (S : sealing Σ).
-  Implicit Types v : val.
 
-  Global Instance to_low_persistent φ : PersistentP (to_low φ).
-  Proof. apply _. Qed.
-  Global Instance to_low_ne n : Proper (ext (dist n) ==> dist n) to_low.
-  Proof. solve_proper. Qed.
-  Global Instance to_low_proper : Proper (ext (≡) ==> (≡)) to_low.
-  Proof. solve_proper. Qed.
-
-  Global Instance from_low_persistent φ : PersistentP (from_low φ).
-  Proof. apply _. Qed.
-  Global Instance from_low_ne n : Proper (ext (dist n) ==> dist n) from_low.
-  Proof. solve_proper. Qed.
-  Global Instance from_low_proper : Proper (ext (≡) ==> (≡)) from_low.
-  Proof. solve_proper. Qed.
-
-  Global Instance is_sealer_unsealer_proper N γ v :
-    Proper (ext (≡) ==> (≡)) (is_sealer_unsealer S N γ v).
+  Global Instance is_sealing_proper γ :
+    Proper (ext (≡) ==> (≡)) (is_sealing S γ).
   Proof.
-    move=>???. apply equiv_dist=>?. apply is_sealer_unsealer_ne=>?.
+    move=>???. apply equiv_dist=>?. apply is_sealing_ne=>?.
     by apply equiv_dist.
   Qed.
-
-  Lemma seal_val N p γ s φ v `{Hφ : ∀ v, PersistentP (φ v)} :
-    {{{ is_sealer_unsealer S N γ s φ ∗ φ v }}} seal SI s v @ p; ⊤
-    {{{ v', RET v'; low v' ∗ is_sealed S N γ v v' }}}.
-  Proof.
-    iIntros (Φ) "#[Hs Hv] HΦ".
-    wp_apply (seal_spec with "Hs"). iIntros (f) "[_ Hf]".
-    wp_apply ("Hf" with "* Hv"). iIntros (v') "Hv'".
-    by iApply ("HΦ" with "Hv'").
-  Qed.
-
-  Lemma unseal_sealed_val N p γ s φ v v' :
-    {{{ is_sealer_unsealer S N γ s φ ∗ is_sealed S N γ v v' }}}
-      unseal SI s v' @ p; ⊤
-    {{{ RET v; φ v }}}.
-  Proof.
-    iIntros (Φ) "#[Hs Hv'] HΦ".
-    wp_apply (unseal_sealed_spec with "Hs"). iIntros (f) "Hf".
-    by wp_apply ("Hf" with "* Hv'").
-  Qed.
-
-  Lemma unseal_low_val N γ s φ v' :
-    {{{ is_sealer_unsealer S N γ s φ ∗ low v' }}} unseal SI s v'
-    ?{{{ v, RET v; φ v }}}.
-  Proof.
-    iIntros (Φ) "#[Hs Hv'] HΦ".
-    wp_apply (unseal_low_spec with "Hs"). iIntros (f) "[_ Hf]".
-    by wp_apply ("Hf" with "* Hv'").
-  Qed.
-End lemmas.
-Typeclasses Opaque to_low from_low.
+End theory.
 End intf.
 
-(** * Morris' dynamic sealing implementation *)
+(** * Dynamic sealing implementation *)
 (**
+	Other than the typecast, this is a transliteration of Morris'
+	implementation of sealing.
+
 	Safe-for-space implementations exist. The sequential code
 <<
 	let r = ref None in
@@ -163,29 +116,27 @@ End intf.
 
 Module code.
 Section code.
-  Context (LI : LockImpl).
+  Context {LI : LockImpl}.
 
-  Definition make_sealer_unsealer : val := λ: <>,
+  Definition make_seal : val := λ: <>,
     let: "tbl" := ref map_empty in
     let: "sync" := make_sync LI () in
-    ("sync", "tbl").
+    let: "seal" := λ: "v" "x",
+      ifloc: "x" as "k" =>
+        "sync" (λ: <>, "tbl" <- map_insert (! "tbl") "k" "v")
+      else abort
+    in
+    let: "unseal" := λ: "f",
+      let: "k" := ref () in
+      "f" "k" ;;
+      "sync" (λ: <>, map_lookup_partial (! "tbl") "k")
+    in
+    ("seal", "unseal").
 
-  Definition seal : val := λ: "p" "v" "x",
-    let: "sync" := Fst "p" in let: "tbl" := Snd "p" in
-    ifloc: "x" as "k" => "sync" (λ: <>, "tbl" <- map_insert (! "tbl") "k" "v")
-    else abort.
-
-  Definition unseal : val := λ: "p" "f",
-    let: "sync" := Fst "p" in let: "tbl" := Snd "p" in
-    let: "k" := ref () in
-    "f" "k" ;;
-    "sync" (λ: <>, map_lookup_partial (! "tbl") "k").
+  Global Instance sealing : SealingImpl := {|
+    intf.make_seal := make_seal
+  |}.
 End code.
-
-Definition sealing (LI : LockImpl) : SealingImpl := {|
-  intf.make_sealer_unsealer := make_sealer_unsealer LI;
-  intf.seal := seal; intf.unseal := unseal
-|}.
 End code.
 
 Module proof.
@@ -199,21 +150,10 @@ Instance subG_sealingΣ {Σ} : subG sealingΣ Σ → sealingG Σ.
 Proof. intros [??]%subG_inv. constructor; apply _. Qed.
 
 Section proof.
-  Context `{heapG Σ, sealingG Σ, LI : LockImpl} (L : lock Σ) (N : namespace).
-  Let SI : SealingImpl := code.sealing LI.
+  Context `{heapG Σ, sealingG Σ, LI : LockImpl} (L : lock Σ).
   Implicit Types l : loc.
   Implicit Types f v : val.
   Notation ext R := (pointwise_relation _ R).
-
-  Let name : Type := gname * loc.
-
-  (**
-	The assertion [is_witness γ k v] represents knowledge that the
-	table underlying the sealer-unsealer pair named [γ] sends
-	location [k] to value [v].
-  *)
-  Definition is_witness (γ : name) (k : loc) (v : val) : iProp Σ :=
-    own (γ.1) (◯ {[k := to_agree v]}).
 
   (**
 	The table underlying the sealer-unsealer pair named [γ] sends
@@ -222,45 +162,57 @@ Section proof.
 	applications of [unseal] are tied to a ghost heap witnessing
 	the table's assignment of a particular value [v] to [k].
 
-	The table can bind locations not tracked by the ghost heap
-	because adversarial code can apply a sealed value to a
+	The table must account for locations not tracked by the ghost
+	heap because adversarial code can apply a sealed value to a
 	low-integrity value [kv]. When [kv] is a location [k], such
-	applications extend the table (but not the ghost heap).
+	applications extend the table, but not the ghost heap.
 
-	We store actual heap resources alongside the ghost heap to
-	ensure we can allocate [is_witness γ k v] given a fresh, high
-	location [k].
+	The assertion [is_witness γ k v] represents knowledge that the
+	ghost heap sends location [k] to value [v] and is used to
+	prove the progressive triple for unsealing. The resource
+	[witness γ m] ties the ghost heap to a sealer-unsealer pair
+	with table contents [m] and heap resources that ensure we can
+	allocate [is_witness γ k v] given a fresh, high location [k].
   *)
-  Definition to_heap : heap → heapUR := fmap to_agree.
 
-  Definition witness (γ : name) (m : heap) : iProp Σ := (
-    ∃ h, ⌜h ⊆ m⌝ ∗ own (γ.1) (● to_heap h) ∗ live (dom _ h) ∗
+  Definition is_witness (γ : gname) (k : loc) (v : val) : iProp Σ :=
+    own γ (◯ {[k := to_agree v]}).
+
+  Definition to_heap : heap → heapUR := fmap to_agree.
+  Definition witness (γ : gname) (m : heap) : iProp Σ := (
+    ∃ h, ⌜h ⊆ m⌝ ∗ own γ (● to_heap h) ∗ live (dom _ h) ∗
     [∗ map] k↦_ ∈ h, k ↦ ()
   )%I.
 
-  Definition tbl_res (γ : name) (φ : val → iProp Σ) : iProp Σ := (
-    ∃ map m, (γ.2) ↦ map ∗ is_map map m ∗ witness γ m ∗
+  Definition tbl_res (l : loc) (γ : gname) (φ : val → iProp Σ) : iProp Σ := (
+    ∃ map m, l ↦ map ∗ is_map map m ∗ witness γ m ∗
     [∗ map] v ∈ m, □ φ v
   )%I.
 
-  Definition is_sealer_unsealer (γ : name) (v : val) φ : iProp Σ := (
-    ∃ sync, ⌜heapN ⊥ N⌝ ∗ heap_ctx ∗ ⌜v = (sync, γ.2)%V⌝ ∗
-    is_sync sync (tbl_res γ φ)
+  Record name : Type := { sync : val; tbl : loc; ghost : gname }.
+  Definition is_sealing (γ : name) φ : iProp Σ :=
+    (heap_ctx ∗ is_sync (sync γ) (tbl_res (tbl γ) (ghost γ) φ))%I.
+
+  Definition is_seal (γ : name) (v : val) : iProp Σ := (
+    ⌜v = LamV "v" (λ: "x",
+      ifloc: "x" as "k" =>
+        (sync γ) (λ: <>, tbl γ <- map_insert (! (tbl γ)) "k" "v")
+      else abort)⌝
   )%I.
 
-  (*
-	The assertion [is_sealed γ v v'] represents knowledge that
-	value [v'] was obtained by sealing value [v] with the
-	sealer-unsealer pair named [γ].
+  Definition is_unseal (γ : name) (v : val) : iProp Σ := (
+    ⌜v = LamV "f" (
+      let: "k" := ref () in
+      "f" "k" ;;
+      (sync γ) (λ: <>, map_lookup_partial (! (tbl γ)) "k"))⌝
+  )%I.
 
-	Unfolding the definition, we have a progressive triple for [v'
-	k] that converts a high, fresh location [k] to a witness
-	[is_witness γ k v] sufficient to ensure that table lookups on
-	[k] will compute [v]
-  *)
   Definition is_sealed (γ : name) (v v' : val) : iProp Σ := (
-    ∀ p k,
-    {{{ k ↦ () ∗ fresh k }}} v' k @ p; ⊤ {{{ RET (); is_witness γ k v }}}
+    ∃ φ, is_sealing γ φ ∗ □ φ v ∗
+    ⌜v' = LamV "x" (
+      ifloc: "x" as "k" =>
+        (sync γ) (λ: <>, tbl γ <- map_insert (! (tbl γ)) "k" v)
+      else abort)%E⌝
   )%I.
 
   (** Structure *)
@@ -270,21 +222,26 @@ Section proof.
   Instance is_witness_timeless γ k v : TimelessP (is_witness γ k v).
   Proof. apply _. Qed.
 
-  Instance tbl_res_ne γ n : Proper (ext (dist n) ==> dist n) (tbl_res γ).
+  Instance tbl_res_ne l γ n : Proper (ext (dist n) ==> dist n) (tbl_res l γ).
   Proof. solve_proper. Qed.
 
-  Global Instance is_sealer_unsealer_persistent γ v φ :
-    PersistentP (is_sealer_unsealer γ v φ).
+  Instance is_sealing_persistent γ φ : PersistentP (is_sealing γ φ).
   Proof. apply _. Qed.
-  Global Instance is_sealer_unsealer_ne γ v n :
-    Proper (ext (dist n) ==> dist n) (is_sealer_unsealer γ v).
-  Proof.
-    (* FIXME: [solve_proper] works but is very slow here *)
-    move=>φ1 φ2 Hφ. preprocess_solve_proper.
-    apply exist_ne. do 4!f_equiv. apply is_sync_ne. f_equiv. by apply Hφ.
-  Qed.
+  Instance is_sealing_ne γ n :
+    Proper (ext (dist n) ==> dist n) (is_sealing γ).
+  Proof. solve_proper. Qed.
 
-  Global Instance is_sealed_persistent γ v v' : PersistentP (is_sealed γ v v').
+  Instance is_seal_persistent γ v : PersistentP (is_seal γ v).
+  Proof. apply _. Qed.
+  Instance is_seal_timeless γ v : TimelessP (is_seal γ v).
+  Proof. apply _. Qed.
+
+  Instance is_unseal_persistent γ v : PersistentP (is_unseal γ v).
+  Proof. apply _. Qed.
+  Instance is_unseal_timeless γ v : TimelessP (is_unseal γ v).
+  Proof. apply _. Qed.
+
+  Instance is_sealed_persistent γ v v' : PersistentP (is_sealed γ v v').
   Proof. apply _. Qed.
 
   (** Ghosts *)
@@ -303,8 +260,8 @@ Section proof.
 
   Lemma witness_high_alloc γ h k v :
     h !! k = None →
-    own (γ.1) (● to_heap h) ==∗
-    own (γ.1) (● to_heap (<[k:=v]> h)) ∗ is_witness γ k v.
+    own γ (● to_heap h) ==∗
+    own γ (● to_heap (<[k:=v]> h)) ∗ is_witness γ k v.
   Proof.
     rewrite /to_heap fmap_insert -own_op=>Hdom.
     apply own_update, auth_update_alloc, alloc_singleton_local_update.
@@ -349,9 +306,8 @@ Section proof.
     rewrite lookup_insert_ne //. by apply map_subseteq_spec.
   Qed.
 
-  Lemma tbl_inv_insert (m : heap) k v (φ : val → iProp Σ)
-      `{Hv : ∀ v, PersistentP (φ v)} :
-    ([∗ map] v ∈ m, □ φ v) -∗ φ v -∗ [∗ map] v ∈ <[k:=v]> m, □ φ v.
+  Lemma tbl_inv_insert (m : heap) k v (φ : val → iProp Σ) :
+    ([∗ map] v ∈ m, □ φ v) -∗ □ φ v -∗ [∗ map] v ∈ <[k:=v]> m, □ φ v.
   Proof.
     iIntros "Hinv #Hv". case Hv': (m !! k) => [v'|].
     - rewrite (big_sepM_insert_override_2 _ _ _ v' v) //.
@@ -359,78 +315,18 @@ Section proof.
     - rewrite big_sepM_insert //. iFrame "Hinv". iAlways. by iFrame "Hv".
   Qed.
 
-  (** Operations *)
+  (** Properties of sealing. *)
 
-(* PDS: We probably do not need heapN ⊥ N after allocation. *)
-  Lemma make_sealer_unsealer_spec p φ `{Hφ : ∀ v, PersistentP (φ v)} :
-    heapN ⊥ N →
-    {{{ heap_ctx }}} make_sealer_unsealer SI () @ p; ⊤
-    {{{ v γ, RET v; is_sealer_unsealer γ v φ }}}.
+  Lemma is_sealed_agree γ v1 v2 v' :
+    is_sealed γ v1 v' -∗ is_sealed γ v2 v' -∗ ⌜v1 = v2⌝.
+  Proof. do 2!iDestruct 1 as (?) "(_&_&%)". by naive_solver. Qed.
+
+  Lemma sealed_high p γ v v' k :
+    {{{ is_sealed γ v v' ∗ k ↦ () ∗ fresh k }}} v' k @ p; ⊤
+    {{{ RET (); is_witness (ghost γ) k v }}}.
   Proof.
-    iIntros (? Φ) "#Hh HΦ". wp_lam. wp_alloc l as "Hl". wp_let.
-      rewrite -wp_fupd. set h := to_heap ∅.
-    iMod (own_alloc (Auth (Excl' h) h)) as (γh) "Hγh"; first done.
-      rewrite (auth_both_op h). iDestruct "Hγh" as "[Hγh _]".
-      set γ : name := (γh, l).
-    iAssert (witness γ ∅) with "[Hγh]" as "Hw".
-    { iExists ∅. iFrame "Hγh".
-      rewrite dom_empty_L big_sepS_empty big_sepM_empty. by auto. }
-    wp_apply (make_sync_spec L _ N (tbl_res γ φ) with "[$Hh Hl Hw]");
-      first done.
-    { iExists map_empty, ∅. iFrame "Hl Hw". rewrite big_sepM_empty. by auto. }
-    iIntros (sync) "Hsync". wp_let.
-    iApply ("HΦ" $! _ γ). iExists sync. by iFrame "% Hh Hsync".
-  Qed.
-
-  Lemma seal_spec p γ s φ `{Hφ : ∀ v, PersistentP (φ v)} :
-    {{{ is_sealer_unsealer γ s φ }}} seal SI s @ p; ⊤ {{{ f, RET f;
-      □ (from_low φ -∗ low f) ∗ ∀ p v,
-      {{{ φ v }}} f v @ p; ⊤ {{{ v', RET v'; low v' ∗ is_sealed γ v v' }}}
-    }}}.
-  Proof.
-    assert (Hbodylow : ∀ (v vk : val),
-      {{{ is_sealer_unsealer γ s φ ∗ φ v ∗ low vk }}}
-        let: "sync" := Fst s in let: "tbl" := Snd s in
-        ifloc: vk as "k" =>
-          "sync" (λ: <>, "tbl" <- ((map_insert ! "tbl") "k") v)
-        else abort
-      ?{{{ v', RET v'; low v' }}}
-    ).
-    { iIntros (v vk Φ) "#(Hs & Hv & Hk) HΦ".
-        iDestruct "Hs" as (sync) "(%&#Hh&%&Hsync)". subst.
-        do 2!(wp_proj; wp_let).
-      wp_typecast Hloc; wp_match; last by wp_apply wp_abort.
-        destruct (is_loc_val _ Hloc) as (k&->). rewrite/is_sync.
-      wp_apply ("Hsync" with "[%]"). iClear "Hsync". iIntros (Ψ) "HR HΨ".
-        iDestruct "HR" as (map m) "(Hl & Hm & Hw & #Hinv)". wp_load.
-      wp_apply (map_insert_spec _ _ _ m with "Hm").
-        iIntros (map') "Hm'". wp_store.
-      iApply ("HΨ" with "[Hl Hm' Hw]"); last by iApply "HΦ"; simpl_low.
-      iExists map', (<[k:=v]> m). iFrame "Hl Hm'". iSplitL.
-      - rewrite (low_val k). by iApply (witness_low with "Hw Hk").
-      - by iApply (tbl_inv_insert with "Hinv Hv"). }
-    iIntros (Φ) "#Hs HΦ". wp_lam.
-    iApply "HΦ". clear p Φ. iSplitL.
-
-    (** Sealing can be low. *)
-    { iIntros "!# #Hφ". rewrite low_rec. iAlways. iNext.
-        iIntros (v Φ) "#Hv HΦ". simpl_subst. wp_value.
-      iApply "HΦ". clear Φ. rewrite low_rec. iAlways. iNext.
-        iIntros (vk Φ) "#Hk HΦ". simpl_subst.
-      wp_apply (Hbodylow with "[$Hs Hφ Hv $Hk] [$HΦ]").
-        rewrite/from_low.
-      by iApply ("Hφ" with "Hv"). }
-    iIntros (p v) "!#". iIntros (Φ) "#Hv HΦ". wp_lam.
-    iApply "HΦ". clear Φ. iSplitL.
-
-    (** Sealed values are low. *)
-    { rewrite low_rec. iAlways. iNext. iIntros (vk Φ) "#Hk HΦ". simpl_subst.
-      by wp_apply (Hbodylow with "[$Hs $Hv $Hk]"). }
-
-    (** Sealed values satisfy [is_sealed]. *)
-    clear p. iIntros (p k) "!#". iIntros (Φ) "[Hk Hf] HΦ". wp_lam.
-      iDestruct "Hs" as (sync) "(%&#Hh&%&Hsync)". subst.
-      do 2!(wp_proj; wp_let).
+    iIntros (Φ) "(Hv' & Hk & Hf) HΦ".
+      iDestruct "Hv'" as (φ) "(#[Hh Hsync] & Hv & %)". subst. wp_lam.
     wp_typecast Hloc; last by exfalso; apply Hloc; exists k.
       wp_match. rewrite/is_sync.
     wp_apply ("Hsync" with "[%]"). iClear "Hsync". iIntros (Ψ) "HR HΨ".
@@ -438,26 +334,126 @@ Section proof.
     wp_apply (map_insert_spec _ _ _ m with "Hm").
       iIntros (map') "Hm'". rewrite -wp_fupd. wp_store.
     iMod (witness_high _ _ k v with "Hh Hw Hk Hf") as "[Hw Hkv]".
-    iApply ("HΨ" with "[Hl Hm' Hw]"); last by iApply ("HΦ" with "Hkv").
+    iApply ("HΨ" with "[Hv Hl Hm' Hw]"); last by iApply ("HΦ" with "Hkv").
     iExists map', (<[k:=v]> m). iFrame "Hl Hm' Hw".
     by iApply (tbl_inv_insert with "Hinv Hv").
   Qed.
 
-  Lemma unseal_sealed_spec p γ s φ :
-    {{{ is_sealer_unsealer γ s φ }}} unseal SI s @ p; ⊤ {{{ f, RET f;
-      ∀ p v v', {{{ is_sealed γ v v' }}} f v' @ p; ⊤ {{{ RET v; φ v }}}
-    }}}.
+  Lemma is_sealed_low γ v v' : is_sealed γ v v' -∗ low v'.
   Proof.
-    iIntros (Φ) "#Hs HΦ". wp_lam.
-    iApply "HΦ". clear p Φ. iIntros (p v v') "!#". iIntros (Φ) "#Hv' HΦ".
-      wp_lam. iDestruct "Hs" as (sync) "(%&#Hh&%&Hsync)". subst.
-      do 2!(wp_proj; wp_let).
-    wp_apply (wp_alloc_fresh with "Hh"); auto.
-      iIntros (k) "[Hk Hf]". wp_let. rewrite/is_sealed.
-    wp_apply ("Hv'" with "* [$Hk $Hf]"). iIntros "Hkv". wp_seq. rewrite/is_sync.
+    iDestruct 1 as (φ) "(#[Hh Hsync] & #Hv & %)". subst. rewrite low_rec.
+      iAlways. iNext. iIntros (vk Φ) "#Hk HΦ". simpl_subst.
+    wp_typecast Hloc; wp_match; last by wp_apply wp_abort.
+      destruct (is_loc_val _ Hloc) as (k&->). rewrite/is_sync.
+    wp_apply ("Hsync" with "[%]"). iClear "Hsync". iIntros (Ψ) "HR HΨ".
+      iDestruct "HR" as (map m) "(Hl & Hm & Hw & #Hinv)". wp_load.
+    wp_apply (map_insert_spec _ _ _ m with "Hm").
+      iIntros (map') "Hm'". wp_store.
+    iApply ("HΨ" with "[Hl Hm' Hw]"); last by iApply "HΦ"; simpl_low.
+    iExists map', (<[k:=v]> m). iFrame "Hl Hm'". iSplitL.
+    - rewrite (low_val k). by iApply (witness_low with "Hw Hk").
+    - by iApply (tbl_inv_insert with "Hinv [Hv]").
+  Qed.
+
+  Lemma is_seal_low γ s φ :
+    is_sealing γ φ -∗ □ (∀ v, low v -∗ φ v) -∗ is_seal γ s -∗ low s.
+  Proof.
+    iIntros "#Hs #Hφ %". subst. rewrite low_rec.
+      iAlways. iNext. iIntros (v Φ) "#Hv HΦ". simpl_subst. wp_value.
+    iApply "HΦ".
+    iApply (is_sealed_low γ v with "[]"). iExists φ. iFrame "Hs".
+    iSplitL; last done. iAlways. by iApply ("Hφ" with "Hv").
+  Qed.
+
+  (** Properties of unsealing. *)
+
+  Lemma unseal_body_low γ v' φ :
+    {{{ is_sealing γ φ ∗ low v' }}}
+      let: "k" := ref () in
+      v' "k" ;;
+      (sync γ) (λ: <>, (map_lookup_partial ! (tbl γ)) "k")
+    ?{{{ v, RET v; φ v }}}.
+  Proof.
+    iIntros (Φ) "(#[Hh Hsync] & #Hv') HΦ".
+    wp_apply (wp_alloc_low with "[$Hh]"); auto; first by simpl_low.
+      iIntros (k) "Hk". wp_let.
+    (* PDS: Hack. *)
+    (*
+     * [wp_on_val_app] should be a Texan triple and there's no call to
+     * state those lemmas in terms of expressions.
+     *)
+    wp_bind (v' k). iDestruct (wp_on_val_app lowloc v' k) as "Happ".
+      rewrite (wp_wand _ _ (v' k)%E _ _).
+    wp_apply ("Happ" with "[Hv'] [Hk]");
+      [by rewrite low_val_eq|by rewrite low_loc on_val_elim|].
+    iIntros (?) "_". wp_seq. iClear "Happ".
+    (* PDS: End hack. *)
+    rewrite/is_sync.
     wp_apply ("Hsync" with "[%]"). iClear "Hsync". iIntros (Ψ) "HR HΨ".
       iDestruct "HR" as (map m) "(Hl & #Hm & Hw & #Hinv)". wp_load.
-      iDestruct (witness_elim with "Hw Hkv") as "%".
+    wp_apply (map_lookup_partial_spec _ _  _ k with "Hm")=>//.
+      iIntros (v'') "%".
+    iApply ("HΨ" with "[Hl Hw]").
+    - iExists map, m. by iFrame "Hl Hm Hw Hinv".
+    - iApply "HΦ". setoid_rewrite always_elim.
+      by rewrite -(big_sepM_lookup (λ _, φ) m k v'').
+  Qed.
+
+  Lemma is_unseal_low γ u φ :
+    is_sealing γ φ -∗ □ (∀ v, φ v -∗ low v) -∗ is_unseal γ u -∗ low u.
+  Proof.
+    iIntros "#Hs #Hφ %". subst. rewrite low_rec.
+      iAlways. iNext. iIntros (v' Φ) "#Hv' HΦ". simpl_subst.
+    wp_apply (unseal_body_low with "[$Hs $Hv']"). iIntros (v) "Hv".
+    iApply "HΦ". by iApply ("Hφ" with "Hv").
+  Qed.
+
+  (** Operations *)
+
+  Lemma make_seal_spec N p φ :
+    heapN ⊥ N →
+    {{{ heap_ctx }}} code.make_seal () @ p; ⊤
+    {{{ v1 v2 γ, RET (v1, v2); is_sealing γ φ ∗ is_seal γ v1 ∗ is_unseal γ v2
+    }}}.
+  Proof.
+    iIntros (? Φ) "#Hh HΦ". wp_lam. wp_alloc l as "Hl". wp_let.
+      rewrite -wp_fupd. set h := to_heap ∅.
+    iMod (own_alloc (Auth (Excl' h) h)) as (γh) "Hγh"; first done.
+      rewrite (auth_both_op h). iDestruct "Hγh" as "[Hγh _]".
+    iAssert (witness γh ∅) with "[Hγh]" as "Hw".
+    { iExists ∅. iFrame "Hγh".
+      rewrite dom_empty_L big_sepS_empty big_sepM_empty. by auto. }
+    wp_apply (make_sync_spec L _ N (tbl_res l γh φ) with "[$Hh Hl Hw]");
+      first done.
+    { iExists map_empty, ∅. iFrame "Hl Hw". rewrite big_sepM_empty. by auto. }
+    iIntros (sync) "#Hsync". set γ := {| sync := sync; tbl := l; ghost := γh |}.
+      do 3!wp_let.
+    iApply ("HΦ" $! _ _ γ). iFrame "Hh Hsync". by auto.
+  Qed.
+
+  Lemma seal_spec p γ s v φ `{!PersistentP (φ v)} :
+    {{{ is_sealing γ φ ∗ is_seal γ s ∗ φ v }}} s v @ p; ⊤
+    {{{ v', RET v'; low v' ∗ is_sealed γ v v' }}}.
+  Proof.
+    iIntros (Φ) "(#Hs & % & #Hv) HΦ". subst. wp_lam. set v' := LamV _ _.
+    iAssert (is_sealed γ v v') as "#Hv'".
+    { iExists φ. iFrame "Hs". iSplitL. by iAlways. done. }
+    iApply "HΦ". iFrame "Hv'".
+    by iApply (is_sealed_low with "Hv'").
+  Qed.
+
+  Lemma unseal_spec p γ u v v' φ :
+    {{{ is_sealing γ φ ∗ is_unseal γ u ∗ is_sealed γ v v' }}} u v' @ p; ⊤
+    {{{ RET v; φ v }}}.
+  Proof.
+    iIntros (Φ) "(#[Hh Hsync] & % & #Hv') HΦ". subst. wp_lam.
+    wp_apply (wp_alloc_fresh with "Hh"); auto.
+      iIntros (k) "[Hk Hf]". wp_let.
+    wp_apply (sealed_high with "[$Hv' $Hk $Hf]"). iIntros "Hwk". wp_seq.
+      rewrite/is_sync.
+    wp_apply ("Hsync" with "[%]"). iClear "Hsync". iIntros (Ψ) "HR HΨ".
+      iDestruct "HR" as (map m) "(Hl & #Hm & Hw & #Hinv)". wp_load.
+      iDestruct (witness_elim with "Hw Hwk") as "%".
     wp_apply (map_lookup_partial_Some_spec _ _ _ _ k with "Hm");
       first done. iIntros "_".
     iApply ("HΨ" with "[Hl Hw]").
@@ -466,60 +462,20 @@ Section proof.
       by iApply (big_sepM_lookup (λ _, φ) m k v with "Hinv").
   Qed.
 
-  Lemma unseal_low_spec p γ s φ :
-    {{{ is_sealer_unsealer γ s φ }}} unseal SI s @ p; ⊤ {{{ f, RET f;
-      □ (to_low φ -∗ low f) ∗ ∀ v', {{{ low v' }}} f v' ?{{{ v, RET v; φ v }}}
-    }}}.
+  Lemma unseal_low_spec γ u v' φ :
+    {{{ is_sealing γ φ ∗ is_unseal γ u ∗ low v' }}} u v' ?{{{ v, RET v; φ v }}}.
   Proof.
-    assert (Hbody : ∀ v',
-      {{{ is_sealer_unsealer γ s φ ∗ low v' }}}
-        let: "sync" := Fst s in let: "tbl" := Snd s in
-        let: "k" := ref () in
-        v' "k" ;;
-        "sync" (λ: <>, (map_lookup_partial ! "tbl") "k")
-      ?{{{ v, RET v; φ v }}}
-    ).
-    { iIntros (v' Φ) "#[Hs Hv'] HΦ".
-        iDestruct "Hs" as (sync) "(%&#Hh&%&Hsync)". subst.
-        do 2!(wp_proj; wp_let).
-      wp_apply (wp_alloc_low with "[$Hh]"); auto; first by simpl_low.
-        iIntros (k) "Hk". wp_let.
-      (* PDS: Hack. *)
-      (*
-       * [wp_on_val_app] should be a Texan triple and there's no call to
-       * state those lemmas in terms of expressions.
-       *)
-      wp_bind (v' k). iDestruct (wp_on_val_app lowloc v' k) as "Happ".
-        rewrite (wp_wand _ _ (v' k)%E _ _).
-      wp_apply ("Happ" with "[Hv'] [Hk]");
-        [by rewrite low_val_eq|by rewrite low_loc on_val_elim|].
-      iIntros (?) "_". wp_seq. iClear "Happ".
-      (* PDS: End hack. *)
-      rewrite/is_sync.
-      wp_apply ("Hsync" with "[%]"). iClear "Hsync". iIntros (Ψ) "HR HΨ".
-        iDestruct "HR" as (map m) "(Hl & #Hm & Hw & #Hinv)". wp_load.
-      wp_apply (map_lookup_partial_spec _ _  _ k with "Hm")=>//.
-        iIntros (v'') "%".
-      iApply ("HΨ" with "[Hl Hw]").
-      - iExists map, m. by iFrame "Hl Hm Hw Hinv".
-      - iApply "HΦ". setoid_rewrite always_elim.
-        by rewrite -(big_sepM_lookup (λ _, φ) m k v''). }
-    iIntros (Φ) "#Hs HΦ". wp_lam.
-    iApply "HΦ". clear Φ. iSplitL.
-    - iIntros "!# #Hφ". rewrite low_rec. iAlways. iNext.
-        iIntros (v' Φ) "Hv' HΦ". simpl_subst.
-        wp_apply (Hbody with "[$Hs $Hv']"). iIntros (v'') "Hv''".
-        iApply "HΦ". rewrite/to_low. by iApply "Hφ".
-    - iIntros (v') "!#". iIntros (Φ) "#Hv' HΦ". wp_lam.
-      wp_apply (Hbody with "[$Hs $Hv'] [$HΦ]").
+    iIntros (Φ) "(#Hs & % & #Hv') HΦ". subst. wp_lam.
+    by wp_apply (unseal_body_low with "[$Hs $Hv'] [$HΦ]").
   Qed.
-End proof.
 
-Definition sealing `{heapG Σ, sealingG Σ, LockImpl}
-    (L : lock Σ) : sealing Σ := {|
-  intf.make_sealer_unsealer_spec := make_sealer_unsealer_spec L;
-  intf.seal_spec := seal_spec;
-  intf.unseal_sealed_spec := unseal_sealed_spec;
-  intf.unseal_low_spec := unseal_low_spec
-|}.
+  Definition sealing : sealing Σ := {|
+    intf.is_seal_low := is_seal_low;
+    intf.is_unseal_low := is_unseal_low;
+    intf.make_seal_spec := make_seal_spec;
+    intf.seal_spec := seal_spec;
+    intf.unseal_spec := unseal_spec;
+    intf.unseal_low_spec := unseal_low_spec
+  |}.
+End proof.
 End proof.
