theories/tests/sealing.v
@@ -1,109 +1,235 @@
 From iris.heap_lang Require Import heap adequacy.
-From iris.heap_lang.lib Require Import sealing.
+From iris.heap_lang.lib Require Import sealing assume.
 From iris.heap_lang.lib Require lock spin_lock.
 From iris.heap_lang Require Import notation proofmode.
 Import sealing.intf.
 
-Local Hint Resolve to_of_val.
+Section lifting.	(* PDS: Hoist. *)
+  Context `{ownPG heap_lang Σ}.
+  Local Hint Resolve to_of_val.
+  Implicit Types n : Z.
+  Implicit Types v : val.
 
-(** * Morris' protected interval manipulating routines *)
+  Lemma wp_stuck_lt_l E v1 v2 Φ :
+    ¬ is_int (of_val v1) → WP v1 ≤ v2 @ E ?{{ Φ }}%I.
+  Proof.
+    move=>Hv1. iApply wp_stuck_bin_op=>//.
+    case: v1 Hv1 => //. case=>//. rewrite/is_int. by naive_solver.
+  Qed.
+
+  Lemma wp_stuck_lt_r E n1 v2 Φ :
+    ¬ is_int (of_val v2) → WP #n1 ≤ v2 @ E ?{{ Φ }}%I.
+  Proof.
+    move=>Hv2. iApply wp_stuck_bin_op=>//.
+    case: v2 Hv2 => //. case=>//. rewrite/is_int. by naive_solver.
+  Qed.
+End lifting.
+
+(** * Protected interval manipulating routines *)
+(**
+	Other than the assertion on unsealing, this is a
+	transliteration of Morris' example.
+*)
 Section intervals_code.
-  Context (SI : SealingImpl).
-
-  Definition make_interval : val := λ: "s" "n1" "n2",
-    seal SI "s" (if: "n1" ≤ "n2" then ("n1", "n2") else ("n2", "n1")).
-
-  Definition unseal' : val := λ: "s" "x",
-    let: "i" := unseal SI "s" "x" in
-    assert: (Fst "i" ≤ Snd "i") ;; "i".
-
-  Definition min : val := λ: "s" "x", Fst (unseal' "s" "x").
-  Definition max : val := λ: "s" "x", Snd (unseal' "s" "x").
-  Definition sum : val := λ: "s" "x" "y",
-      let: "i" := unseal' "s" "x" in
-      let: "j" := unseal' "s" "y" in
-      seal SI "s" (Fst "i" + Fst "j", Snd "i" + Snd "j").
-
-  Definition use : val := λ: "s" <>,
-    let: "i" := unseal' "s" (make_interval "s" #0 #10) in
-    assert: Fst "i" = #0 ;;
-    assert: Snd "i" = #10.
+  Context {SI : SealingImpl}.
 
   Definition intervals : expr :=
-    let: "s" := make_sealer_unsealer SI () in
-    (use "s", make_interval "s", min "s", max "s", sum "s").
+    let: "p" := make_seal () in
+    let: "seal" := Fst "p" in let: "unseal" := Snd "p" in
+    let: "unseal" := λ: "x",
+      let: "i" := "unseal" "x" in assert: (Fst "i" ≤ Snd "i") ;; "i"
+    in
+    let: "make_int" := λ: "n1" "n2",
+      "seal" (if: "n1" ≤ "n2" then ("n1", "n2") else ("n2", "n1"))
+    in
+    let: "min" := λ: "x", Fst ("unseal" "x") in
+    let: "max" := λ: "x", Snd ("unseal" "x") in
+    let: "sum" := λ: "x" "y",
+      let: "i" := "unseal" "x" in
+      let: "j" := "unseal" "y" in
+      "seal" (Fst "i" + Fst "j", Snd "i" + Snd "j")
+    in ("make_int", "min", "max", "sum").
 End intervals_code.
 
-(**
-	We prove a pair of triples for each operation, for use with
-	high- and low-integrity code. For each pair, we could factor
-	out a shared verification condition, but that's not worth
-	doing with proofs this short.
-*)
 Section intervals_proof.
   Context `{heapG Σ, SI : SealingImpl} (S : sealing Σ) (N : namespace).
   Implicit Types f v : val.
   Implicit Types n : Z.
 
-  Definition is_interval' (n1 n2 : Z) (v : val) : iProp Σ :=
+  Definition is_int' (n1 n2 : Z) (v : val) : iProp Σ :=
     (⌜v = (#n1, #n2)%V⌝ ∗ ⌜n1 ≤ n2⌝)%I.
 
-  Global Instance is_interval'_persistent n1 n2 v :
-    PersistentP (is_interval' n1 n2 v).
+  Instance is_int'_persistent n1 n2 v :
+    PersistentP (is_int' n1 n2 v).
   Proof. apply _. Qed.
 
-  Definition is_interval_sealer (γ : name S) (s : val) : iProp Σ :=
-    is_sealer_unsealer S N γ s (λ v, (∃ n1 n2, is_interval' n1 n2 v))%I.
+  Notation intφ := (λ v, (∃ n1 n2, is_int' n1 n2 v))%I (only parsing).
+  Instance intφ_persistent v : PersistentP (intφ v).
+  Proof. apply _. Qed.
 
-  Definition is_interval (γ : name S) (n1 n2 : Z) (v : val) : iProp Σ :=
-    is_sealed S N γ (#n1, #n2)%V v.
+  Record ctx : Type := { γ : name S; seal : val; unseal : val }.
 
-  Lemma make_interval_spec p γ s :
-    {{{ is_interval_sealer γ s }}} make_interval SI s @ p; ⊤
-    {{{ f1, RET f1; ∀ p n1,
-      {{{ True }}} f1 #n1 @ p; ⊤ {{{ f2, RET f2; ∀ p n2,
-        {{{ True }}} f2 #n2 @ p; ⊤
-        {{{ v, RET v; low v ∗ is_interval γ (Z.min n1 n2) (Z.max n1 n2) v }}}
-      }}}
+  Definition int_ctx (ctx : ctx) : iProp Σ := (
+    is_sealing S (γ ctx) intφ ∗
+    is_seal S (γ ctx) (seal ctx) ∗
+    is_unseal S (γ ctx) (unseal ctx)
+  )%I.
+
+  Definition is_interval (ctx : ctx) (n1 n2 : Z) (v : val) : iProp Σ :=
+    (is_sealed S (γ ctx) (#n1, #n2)%V v)%I.
+
+  (** The make interval function. *)
+
+  Definition is_make_int (ctx : ctx) (v : val) : iProp Σ := (
+    ⌜v = LamV "n1" (λ: "n2",
+      (seal ctx) (if: "n1" ≤ "n2" then ("n1", "n2") else ("n2", "n1")))⌝
+  )%I.
+  Definition is_make_int_2 (ctx : ctx) (n1 : Z) (v : val) : iProp Σ := (
+    ⌜v = LamV "n2" (
+      (seal ctx) (if: #n1 ≤ "n2" then (#n1, "n2") else ("n2", #n1)))%E⌝
+  )%I.
+  Definition make_int_body ctx (e1 e2 : expr) : expr :=
+    ((seal ctx) (if: e1 ≤ e2 then (e1, e2) else (e2, e1)))%E.
+  Notation MkInt ctx v n1 n2 := (
+    low v%V ∗ is_interval ctx (Z.min n1 n2) (Z.max n1 n2) v
+  )%I (only parsing).
+
+  Lemma make_int_body_nn p ctx n1 n2 :
+    {{{ int_ctx ctx }}} make_int_body ctx (#n1) (#n2) @ p; ⊤
+    {{{ v, RET v; MkInt ctx v n1 n2 }}}.
+  Proof.
+    iIntros (Φ) "#(HS&Hs&Hu) HΦ".
+      rewrite/make_int_body/is_interval/is_int'.
+    wp_op=>[?|/Z.lt_le_incl ?]; wp_if; wp_apply (seal_spec with "[$HS $Hs]").
+    - by iExists n1, n2; auto. by rewrite (Z.min_l n1) // (Z.max_r _ n2).
+    - by iExists n2, n1; auto. by rewrite (Z.min_r _ n2) // (Z.max_l n1).
+  Qed.
+
+  Lemma make_int_body_nv ctx n1 v2 :
+    {{{ int_ctx ctx }}} make_int_body ctx (#n1) v2
+    ?{{{ v n2, RET v; MkInt ctx v n1 n2 }}}.
+  Proof.
+    iIntros (Φ) "Hctx HΦ". rewrite/make_int_body.
+    case: (decide (is_int (of_val v2)))=>Hv2; last by wp_apply wp_stuck_lt_r.
+      destruct (is_int_val _ Hv2) as (n2&->).
+    wp_apply (make_int_body_nn with "Hctx"). iIntros (v) "Hv".
+    by iApply ("HΦ" $! _ n2 with "Hv").
+  Qed.
+
+  Lemma make_int_body_vv ctx v1 v2 :
+    {{{ int_ctx ctx }}} make_int_body ctx v1 v2
+    ?{{{ v n1 n2, RET v; MkInt ctx v n1 n2 }}}.
+  Proof.
+    iIntros (Φ) "Hctx HΦ". rewrite/make_int_body.
+    case: (decide (is_int (of_val v1)))=>Hv1; last by wp_apply wp_stuck_lt_l.
+      destruct (is_int_val _ Hv1) as (n1&->).
+    wp_apply (make_int_body_nv with "Hctx"). iIntros (v n2) "Hv".
+    by iApply ("HΦ" $! _ n1 with "Hv").
+  Qed.
+
+  Lemma make_int_2_spec p ctx mk n1 n2 :
+    {{{ int_ctx ctx ∗ is_make_int_2 ctx n1 mk }}} mk #n2 @ p; ⊤
+    {{{ v, RET v; MkInt ctx v n1 n2 }}}.
+  Proof.
+    iIntros (Φ) "[Hctx %] HΦ". subst. wp_lam.
+    by wp_apply (make_int_body_nn with "Hctx [$HΦ]").
+  Qed.
+
+  (* PDS: Annoying without [make_int_any_spec]. *)
+  Lemma make_int_2_any_spec ctx mk n1 v2 :
+    {{{ int_ctx ctx ∗ is_make_int_2 ctx n1 mk }}} mk v2
+    ?{{{ v n2, RET v; MkInt ctx v n1 n2 }}}.
+  Proof.
+    iIntros (Φ) "[Hctx %] HΦ". subst. wp_lam.
+    by wp_apply (make_int_body_nv with "Hctx [$HΦ]").
+  Qed.
+
+  Lemma make_int_2_low_spec ctx mk n1 :
+    int_ctx ctx -∗ is_make_int_2 ctx n1 mk -∗ low mk.
+  Proof.
+    iIntros "#Hctx %". subst. rewrite low_rec. iAlways. iNext.
+    iIntros (v2 Φ) "_ HΦ". simpl_subst.
+    wp_apply (make_int_body_nv with "Hctx"). iIntros (v ?) "[Hv _]".
+    by iApply ("HΦ" with "Hv").
+  Qed.
+
+  Lemma make_int_spec p ctx mk n1 :
+    {{{ int_ctx ctx ∗ is_make_int ctx mk }}} mk #n1 @ p; ⊤
+    {{{ f, RET f; is_make_int_2 ctx n1 f }}}.
+  Proof. iIntros (Φ) "[Hctx %] HΦ". subst. wp_lam. by iApply "HΦ". Qed.
+
+  Lemma make_int_any_spec p ctx mk v1 :
+    {{{ int_ctx ctx ∗ is_make_int ctx mk }}} mk v1 @ p; ⊤
+    {{{ f n1, RET f; is_make_int_2 ctx n1 f }}}.
+  Proof.
+    iIntros (Φ) "[Hctx %] HΦ". subst. wp_lam. (* no progress *)
+  Abort.
+
+  Lemma make_int_low_spec ctx mk :
+    int_ctx ctx -∗ is_make_int ctx mk -∗ low mk.
+  Proof.
+    iIntros "#Hctx %". subst. rewrite low_rec. iAlways. iNext.
+    iIntros (v1 Φ) "_ HΦ". simpl_subst. wp_value.
+    iApply "HΦ". clear Φ. rewrite low_rec. iAlways. iNext.
+    iIntros (v2 Φ) "_ HΦ". simpl_subst.
+    wp_apply (make_int_body_vv with "Hctx"). iIntros (v ??) "[Hv _]".
+    by iApply ("HΦ" with "Hv").
+  Qed.
+
+  Lemma make_int_val_spec p ctx mk n1 n2 :
+  {{{ int_ctx ctx ∗ is_make_int ctx mk }}} mk #n1 #n2 @ p; ⊤
+  {{{ v, RET v; MkInt ctx v n1 n2 }}}.
+  Proof.
+    iIntros (Φ) "[#Hctx Hmk] HΦ".
+    wp_apply (make_int_spec with "[$Hctx $Hmk]"). iIntros (f) "Hf".
+    by wp_apply (make_int_2_spec with "[$Hctx $Hf] [$HΦ]").
+  Qed.
+
+  (** The unseal function. *)
+
+  Lemma unseal_spec p γ s :
+    {{{ is_interval_sealer γ s }}} unseal' SI s @ p; ⊤ {{{ f, RET f; ∀ p n1 n2 v',
+      {{{ is_interval γ n1 n2 v' }}} f v' @ p; ⊤ {{{ RET (#n1, #n2); ⌜n1 ≤ n2⌝ }}}
     }}}.
   Proof.
     iIntros (Φ) "#Hs HΦ". wp_lam.
-    iApply "HΦ". clear p Φ. iIntros (p n1) "!#". iIntros (Φ) "_ HΦ". wp_lam.
-    iApply "HΦ". clear p Φ. iIntros (p n2) "!#". iIntros (Φ) "_ HΦ". wp_lam.
-    wp_apply (seal_spec with "Hs"). iIntros (f) "[_ Hf]".
-    rewrite/is_interval/is_interval'. wp_op=>[?|/Z.lt_le_incl ?]; wp_if.
-    - rewrite (Z.min_l n1) // (Z.max_r _ n2) //.
-      wp_apply ("Hf" with "* [] [$HΦ]"). by iExists n1, n2; auto.
-    - rewrite (Z.min_r _ n2) // (Z.max_l n1) //.
-      wp_apply ("Hf" with "* [] [$HΦ]"). by iExists n2, n1; auto.
+    iApply "HΦ". clear p Φ. iIntros (p n1 n2 v') "!#". iIntros (Φ) "Hv' HΦ".
+      wp_lam.
+   wp_apply (unseal_sealed_val with "[$Hs $Hv']").
+      iDestruct 1 as (n'1 n'2) "[EQ %]". iDestruct "EQ" as %[=<-<-]. wp_let.
+      do 2!wp_proj. wp_op=>?; last by exfalso; lia.
+    wp_apply wp_assert. iSplit; first done. iNext. wp_seq.
+    by iApply ("HΦ" with "[%]").
   Qed.
 
-  Lemma make_interval_low_spec p γ s :
-    {{{ is_interval_sealer γ s }}} make_interval SI s @ p; ⊤
-    {{{ f, RET f; low f }}}.
-  Proof.
-    iIntros (Φ) "#Hs HΦ". wp_lam.
-    iApply "HΦ". clear p Φ. rewrite low_rec. iAlways. iNext.
-    iIntros (v1 Φ) "#Hv1 HΦ". simpl_subst. wp_value.
-    iApply "HΦ". clear Φ. rewrite low_rec. iAlways. iNext.
-    iIntros (v2 Φ) "#Hv2 HΦ". simpl_subst.
-    wp_apply (seal_spec with "Hs"). iIntros (f) "[_ Hf]".
-    (* Inlining (derived) rules for stuck ≤. *)
-    wp_bind (_ ≤ _)%E. case: (decide (is_int (of_val v1)))=>Hv1; last first.
-    { iApply wp_stuck_bin_op=>//.
-      case: v1 Hv1 => //. case=>//. rewrite/is_int. by naive_solver. }
-    destruct (is_int_val _ Hv1) as (n1&->).
-    case: (decide (is_int (of_val v2)))=>Hv2; last first.
-    { iApply wp_stuck_bin_op=>//.
-      case: v2 Hv2 => //. case=>//. rewrite/is_int. by naive_solver. }
-    destruct (is_int_val _ Hv2) as (n2&->).
-    (* Reasoning about the body. *)
-    rewrite/is_interval/is_interval'. wp_op=>[?|/Z.lt_le_incl ?]; wp_if.
-    - wp_apply ("Hf" with "* [] [HΦ]"). by iExists n1, n2; auto.
-      by iIntros (?) "[? _]"; iApply "HΦ"; iFrame.
-    - wp_apply ("Hf" with "* [] [HΦ]"). by iExists n2, n1; auto.
-      by iIntros (?) "[? _]"; iApply "HΦ"; iFrame.
-  Qed.
+  (** The min function. *)
+
+  Definition is_min (ctx : ctx) (v : val) : iProp Σ := (
+    ⌜v = LamV "x" (Fst ((unseal ctx) "x"))⌝
+  )%I.
+
+  Definition is_max (ctx : ctx) (v : val) : iProp Σ := (
+    ⌜v = LamV "x" (Snd ((unseal ctx) "x"))⌝
+  )%I.
+
+  Definition is_sum (ctx : ctx) (v : val) : iProp Σ := (
+    ⌜v = LamV "x" (λ: "y",
+      let: "i" := (unseal ctx) "x" in
+      let: "j" := (unseal ctx) "y" in
+      (seal ctx) (Fst "i" + Fst "j", Snd "i" + Snd "j"))⌝
+  )%I.
+
+  Definition is_sum_2 (ctx : ctx) (x : val) (v : val) : iProp Σ := (
+    ⌜v = LamV "y" (
+      let: "i" := (unseal ctx) x in
+      let: "j" := (unseal ctx) "y" in
+      (seal ctx) (Fst "i" + Fst "j", Snd "i" + Snd "j"))⌝
+  )%I.
+
+
+
+
+
 
   Lemma unseal'_spec p γ s :
     {{{ is_interval_sealer γ s }}} unseal' SI s @ p; ⊤ {{{ f, RET f; ∀ p n1 n2 v',
@@ -305,6 +431,24 @@ Section intervals_proof.
   Qed.
 End intervals_proof.
 
+Section intervals_client_code.
+  Context {SI : SealingImpl}.
+
+  Definition interval_client : expr :=
+    let: "p" := intervals in
+    let: "make_int" := Fst $ Fst $ Fst "p" in
+    let: "min" := Snd $ Fst $ Fst "p" in
+    let: "max" := Snd $ Fst "p" in
+    let: "sum" := Snd "p" in
+    let: "i100" := "sum" ("make_int" #1 #0) ("make_int" #(-1) #100) in
+    let: <> := assert: "min" "i0" = #0 in
+    let: "use" := λ: "i",
+      assert: ("min" "i" ≤ "max" "i") ;;
+      "sum" "i" "i100"
+    in
+    ("use", "p").
+End intervals_client_code.
+
 (** * Public-key interfaces for sealer-unsealer pairs *)
 (**
 	When instantiated with suitable representation invariants,
@@ -324,15 +468,23 @@ Section pk_proof.
   Implicit Types f v : val.
   Implicit Types n : Z.
 
-  Definition is_sign (φ : val → iProp Σ) (sign : val) : iProp Σ :=
-    (∀ p v, {{{ φ v }}} sign v @ p; ⊤ {{{ v', RET v'; low v' }}})%I.
-  Definition is_verify (φ : val → iProp Σ) (verify : val) : iProp Σ :=
-    (∀ v', {{{ low v' }}} verify v' ?{{{ v, RET v; φ v }}})%I.
+  Section sig_triples.
+    Context (φ : val → iProp Σ) (sig : val → val → iProp Σ).
+    Definition is_sign (sign : val) : iProp Σ := (∀ p v,
+      {{{ φ v }}} sign v @ p; ⊤ {{{ v', RET v'; low v' ∗ □ sig v v' }}}
+    )%I.
+    Definition verify_sig (verify : val) : iProp Σ :=
+      (∀ v v', {{{ sig v v' }}} verify v' {{{ RET v; φ v }}})%I.
+    Definition verify_low (verify : val) : iProp Σ :=
+      (∀ v', {{{ low v' }}} verify v' ?{{{ v, RET v; φ v }}})%I.
+    Definition is_verify (v : val) : iProp Σ :=
+      (low v ∗ verify_sig v ∗ verify_low v)%I.
+  End sig_triples.
 
   Lemma signature_scheme_spec p φ `{Hφ : ∀ v, PersistentP (φ v)} :
     heapN ⊥ N →
     {{{ heap_ctx ∗ to_low φ }}} make_key_pair () @ p; ⊤
-    {{{ v1 v2, RET (v1, v2); low v2 ∗ is_sign φ v1 ∗ is_verify φ v2 }}}.
+    {{{ v1 v2 sig, RET (v1, v2); is_sign φ sig v1 ∗ is_verify φ sig v2 }}}.
   Proof.
     iIntros (? Φ) "#[Hh Hφ] HΦ". wp_lam.
     wp_apply (make_sealer_unsealer_spec S N _ φ with "Hh");
@@ -340,7 +492,16 @@ Section pk_proof.
     wp_apply (seal_spec with "Hk"). iIntros (sign) "[_ #Hsign]".
     wp_apply (unseal_low_spec with "Hk").
       iIntros (verify) "[Hvlow #Hverify]". wp_value.
-    iApply "HΦ". iFrame "Hverify".
+    iApply ("HΦ" $! _ _ (is_sealed S N γ)). clear p Φ. iSplitR.
+    { iIntros (p v) "!#". iIntros (Φ) "Hv HΦ".
+      wp_apply ("Hsign" with "* Hv"). iIntros (v') "[Hv'l #Hv's]".
+      iApply ("HΦ" with "[$Hv'l Hv's]"). by iAlways. }
+    iSplitL.
+    { by iApply ("Hvlow" with "Hφ"). }
+    iFrame "Hverify".
+    - iSplitL.
+      by iApply "HΦ".
+    iFrame "Hverify".
     iSplitL; first by iApply ("Hvlow" with "Hφ").
     clear p Φ. iIntros (p v) "!#". iIntros (Φ) "Hv HΦ".
     wp_apply ("Hsign" with "* Hv"). iIntros (?) "[? _]".
@@ -370,6 +531,42 @@ Section pk_proof.
     by iApply "HΦ".
   Qed.
 End pk_proof.
+
+(** * Simple security protocol *)
+(**
+	The following example regards its context as an adversarial
+	network. The send and receive functions transmit
+	high-integrity locations containing even numbers.
+*)
+Section proto_code.
+  Context {SI : SealingImpl}.
+
+  Definition protocol : expr :=
+    let: "k" := make_key_pair () in
+    let: "sign" := Fst "k" in let: "verify" := Snd "k" in
+    let: "k" := make_key_pair () in
+    let: "enc" := Fst "k" in let: "dec" := Snd "k" in
+    let: "send" := λ: "x", assume: even: "x" ;; "sign" ("enc" (ref "x")) in
+    let: "recv" := λ: "m", assert: even: ! ("dec" ("verify" "m")) in
+    ("send", "recv").
+End proto_code.
+
+Section proto_proof.
+  Context `{heapG Σ, SI : SealingImpl} (S : sealing Σ) (N : namespace).
+  Implicit Types f v : val.
+  Implicit Types n : Z.
+  Implicit Types l : loc.
+
+  Let φenc (v : val) : iProp Σ := (∃ l n, ⌜v = l%V⌝ ∗ l ↦ #n ∗ ⌜Z.even n⌝)%I.
+  Let φsign (v' : val) : iProp Σ := (
+    ∃ v,
+  )%I.
+  Lemma protocol_spec N :
+    heapN ⊥ N →
+    {{{ heap_ctx }}} protocol {{{ v, RET v; low v }}}.
+  Proof.
+    iIntros (Φ) "HΦ". rewrite/protocol.
+    wp_apply (signature_scheme_spec with "
 
 (*
 	PDS: We need a signature/encryption scheme client.
